\documentclass[a4paper,12pt]{article}
\usepackage[a4paper,top=1.0cm, bottom=1.5cm, left=1.2cm, right=1.2cm]{geometry}

\usepackage[T2A]{fontenc}			
\usepackage[utf8]{inputenc}		
\usepackage[english,russian]{babel}	
\usepackage{amsmath,amsfonts,amssymb,amsthm,mathtools} 
\usepackage{wasysym}
\usepackage{graphicx}
\usepackage{wrapfig}
\usepackage{hyperref}
\usepackage{subcaption}
\DeclareGraphicsExtensions{.pdf, .png, .jpg}

\begin{document}
 
\begin{enumerate}
	\item $f(X) = \det(X^{-1}+A)$, $\nabla_X f$ --- ?
	$$[D_X f](h) = \langle\nabla_X f, h\rangle = [D_{X^{-1} + A} \det(X^{-1}+A)]([D_X X^{-1}](h))$$
	$$[D_Y \det(Y)](h) = \left\langle\left(\frac{\partial \det(Y)}{\partial y_{ij}}\right)_{ij}, h\right\rangle = \left\langle\left(\frac{\partial\left(\sum\limits_{k}(y_{ik}(-1)^{k+i}M_{ik})\right)}{\partial y_{ij}}\right)_{ij}, h\right\rangle = \left\langle\left((-1)^{i+j}M_{ij}\right)_{ij}, h\right\rangle = $$
	$$=\biggr/Y^{-1} = \frac{1}{\det Y} ((-1)^{i+j}M_{ji})_{ij}\biggr/= \left\langle \det Y\cdot Y^{-T}, h\right\rangle$$
	$$0 = [D_X I](h) = [D_X (XX^{-1})](h) = X[D_X X^{-1}](h) + [D_X X](h)X^{-1}$$ 
	$$\Longrightarrow [D_X X^{-1}](h) = -X^{-1}[D_X X](h)X^{-1} = -X^{-1}hX^{-1}$$
	$$[D_X f](h) = -\left\langle \det Y\cdot Y^{-T}, X^{-1}hX^{-1}\right\rangle = -\det Y\cdot\text{tr}(Y^{-1}X^{-1}hX^{-1}) = -\det Y\cdot\text{tr}(X^{-1}Y^{-1}X^{-1}h)=$$
	$$=-\det (X^{-1}+A)\cdot\text{tr}(X^{-1}(X^{-1}+A)^{-1}X^{-1}h)$$
	$$\Longrightarrow \nabla_X f = -\det(X^{-1}+A)\cdot \left(X^{-1}(X^{-1}+A)^{-1}X^{-1}\right)^T = -\det(X^{-1}+A)\cdot X^{-T}(X^{-1}+A)^{-T}X^{-T}$$
	
	\item 
	\begin{enumerate}
		\item $f(t) = \|(A + tI_n)^{-1}b\|$
		$$\frac{\partial}{\partial t}\|(A + tI_n)^{-1}b\| = \frac{b^T(A + tI_n)^{-T}}{\|(A + tI_n)^{-1}b\|}\frac{\partial}{\partial t}(A + tI_n)^{-1}b= -\frac{b^T(A + tI_n)^{-T}}{\|(A + tI_n)^{-1}b\|}(A + tI_n)^{-1}(A + tI_n)^{-1}b$$
		$$ \frac{\partial^2f}{\partial t^2} = -\frac{\partial}{\partial t}\frac{b^T(A + tI_n)^{-T}}{\|(A + tI_n)^{-1}b\|}(A + tI_n)^{-1}(A + tI_n)^{-1}b = \frac{\left[b^T(A + tI_n)^{-T}(A + tI_n)^{-1}(A + tI_n)^{-1}b\right]^2}{\|(A + tI_n)^{-1}b\|^3} + $$
		$$+ \frac{b^T}{\|(A + tI_n)^{-1}b\|}(A + tI_n)^{-T}(A + tI_n)^{-T}(A + tI_n)^{-1}(A + tI_n)^{-1}b +$$
		$$+ \frac{b^T(A + tI_n)^{-T}}{\|(A + tI_n)^{-1}b\|}(A + tI_n)^{-1}(A + tI_n)^{-1}(A + tI_n)^{-1}b$$
		
		\item $f(x) = \frac{1}{2}\|xx^T - A\|^2 $
		$$\frac{\partial}{\partial x}\frac{1}{2}\|xx^T - A\|^2 = \frac{\partial}{\partial x^k}\frac{1}{2}\left((x_ix_j - A_{ij}) \cdot(x^jx^i - A^{ij})\right) = $$
		$$=\frac{1}{2}((\delta_i^kx_j + \delta^k_jx_i)(x^jx^i - A^{ji}) +(x_ix_j - A_{ij})(\delta^{kj}x^i + \delta^{ik}x^j)) =2\|x\|^2x^T - 2x^T A^T$$
		$$\frac{\partial^2f}{\partial x^l\partial x^k} = 2\delta^{kl} x_j x^j + 4x^k x^l - 2A^{kl} = 2I\|x\|^2 + 4xx^T - 2A$$
	\end{enumerate}

\item 
	\begin{enumerate}
		\item[$\nabla_b L$]
		$$D_xL[dx] = \langle\nabla_x L; dx\rangle~~~~~D_bL[db] = \langle\nabla_b L; db\rangle = D_xL[D_bX[db]] = \langle\nabla_x L; A^{-1}db\rangle = \langle A^{-T}\nabla_x L; db\rangle$$
			$$\Longrightarrow \nabla_b L = A^{-T}\nabla_x L$$
		
		\item[$\nabla_A L$]
		
		$$D_aL[dA] = D_xL[D_AX[dA]] = \langle\nabla_x L; -A^{-1}dAA^{-1}b\rangle = \langle-A^{-T}\nabla_x L; dAA^{-1}b\rangle = $$
		$$ = \langle-A^{-1}bA^{-T}\nabla_x L; dA\rangle \Longrightarrow \nabla_AL = - A^{-1}bA^{-T}\nabla_x L$$
	\end{enumerate}

\end{enumerate}

	
\end{document}